## 25.1
$$
|\mu_{0}| = |g| \frac{\mu_{B}^{e}}{\hbar} |S| = |g| \frac{2}{2m_{e}} = 2 \frac{e}{2m_{e}}|S|
$$
$$
|\mu_{p}| = |g| \frac{\mu_{B}^{p}}{\hbar} |S| = |g| \frac{2}{2m_{p}} = 5.6 \frac{e}{2m_{p}}|S|
$$
$$
\frac{|\mu_{e}|}{|\mu_{p}|} = \frac{2m_{p}}{5.6m_{e}} = \frac{2}{5.6} \frac{1.67E-27}{9.09E-31} =660
$$

## 25.2 
For spin up
$$
\cos \theta = \frac{\frac{1}{2}\hbar}{\sqrt{ \frac{1}{2}\left( \frac{1}{2}+1 \right)\hbar }} = \frac{1}{\sqrt{ 3 }} \implies \theta = 54.7^{\circ}
$$
For spin down 
$$
\cos \theta = \frac{-\frac{1}{2}\hbar}{\sqrt{ \frac{1}{2}\left( \frac{1}{2}+1 \right)\hbar }} = \frac{-1}{\sqrt{ 3 }} \implies \theta = 125.3^{\circ}
$$
## 25.3
$$
g=-2
$$
$$
\hat{H} = -\hat{\mu}_{e} \cdot B = -(\hat{\mu}_{e})_{z}B_{z}=-\frac{geB_{z}}{2m_{0}}\hat{S}_{z}=\omega_{0}\hat{S}_{z}
$$
Eigenvalues: 
$$
+\frac{\hbar\omega_{0}}{2}, \ -\frac{\hbar\omega_{0}}{2}
$$
$$
\Delta E = \hbar \omega_{0} =\frac{2eB_{z}\hbar}{2m_{0}} = \frac{2\times 1.6E-19 \times_{1}\times \hbar}{2 \times 9.1E-31}
$$
$$
\omega_{0}=1.76E11
$$
$$
\lambda = \frac{2mc}{\omega_{0}}=\frac{2\pi\times3E8}{1.76E11} = 1.1cm 
$$

## 25.4
Prove $[\hat{S}_{x}, \ \hat{S}_{y}] =i\hbar \hat{S}_{z}$

$$
[\hat{S}_{x}, \hat{S}_{y}] = \hat{S}_{x}\hat{S}_{y} - \hat{S}_{y}\hat{S}_{x}
$$
$$
=\frac{\hbar}{2}\begin{pmatrix}0 & 1\\1 & 0\end{pmatrix} \frac{\hbar}{2}\begin{pmatrix}0 & -i\\i & 0\end{pmatrix} -\frac{\hbar}{2}\begin{pmatrix}0 & -i\\i & 0\end{pmatrix}\frac{\hbar}{2}\begin{pmatrix}0 & 1\\1 & 0\end{pmatrix}
$$
$$
-\frac{\hbar^{2}}{2}\begin{pmatrix}0 & i\\-i & 0\end{pmatrix} = i\hbar \hat{S}_{z}
$$





