---
dg-publish: true
---
## Spherical Coordinates and the Lagrangian
$$
x = r\cos \phi \sin \theta
$$
$$
y = r\sin \phi \sin \theta
$$
$$
z = r\cos \theta
$$
Energy:
$$
T=\frac{1}{2}m
(\dot{x}^{2}+\dot{y}^{2}+\dot{z}^{2})
$$
$$
\frac{d}{dt} \frac{\partial L}{\partial \dot{q}i}-\frac{\partial L}{\partial {q}i}=0
$$
NB: what depends on time? all 3!
![[Pasted image 20240126081355.png]]

$$
\dot{z} =\frac{d}{dt} z=\frac{d}{dt} (r\cos\theta) = \dot{r}\cos\theta+ r(-\sin(\theta)\dot{\theta})
$$
$$
=\dot{r}\cos \theta-r \dot{\theta}\sin \theta
$$
### Recall steps to solve Lagrangian (5)
1. Find T
2. Find U
3. "Calculate" L = T-U
4. Euler-Lagrange equation
$$
\frac{d}{dt} \frac{dL}{d\dot{q}_{i}} - \frac{dL}{dq_{i}}=0
$$
5. Solve resulting diff eq. 

### Examples:
Harmonic Oscillator
Setup: wall with spring, mass attached to spring
position is defined as $x$
Equilibrium length of spring is $x_{0}$ with spring constant $k$
$$
T = \frac{1}{2} m\dot{x}^{2}
$$
$$
U = \frac{1}{2}k(x-x_{0})^{2}
$$
$$
L = T-U = \frac{1}{2}m\dot{x}^{2} - \frac{1}{2}k(x-x_{0})^{2}
$$
$$
L=\frac{1}{2}(m\dot{x}^{2}-k(x^{2}-2x_{0}x+x_{0}^{2}))
$$
$$
L = \frac{1}{2}(m\dot{x}^{2}-kx^{2}-2x_{0}x+x_{0}^{2})
$$
Usually pick that $x_{0}$ is 0 and start measurements from that point. This is different

Do Euler-Lagrange 
$$
\frac{d}{dt} \frac{\partial L}{\partial \dot{x}} - \frac{\partial L}{dx}=0
$$
$$
\frac{\partial L}{\partial \dot{x}} = m\dot{x}
$$
$$
 \frac{d}{dt} (m\dot{x})=m\dot{x}
$$
$$
\frac{\partial L}{\partial x} = -k(x-x_{0})
$$
$$
m\ddot{x} + k(x-x_{0})=0
$$
$$
\ddot{x}=-\frac{k}{m}(x-x_{0})
$$
What we expect
Solution:
$$
Ae^{i\omega t}+Be^{-i\omega t}
$$
or sin/cos depending on your preference
Harmonic Oscillator + Gravity
Vertically hanging harmonic oscillator

$$
T = \frac{1}{2}m\dot{x}^{2}
$$
$$
U = \frac{1}{2} k(x-x_{0})^{2}+mgx
$$
$$
L = T - U = \frac{1}{2}m\dot{x}^{2} - \frac{1}{2}k(x-x_{0})^{2}-mgx
$$
$$
\frac{\partial L}{\partial \dot{x}} = m\dot{x}
$$
$$
\frac{d}{dt} \frac{\partial L}{\partial \dot{x}} = m\ddot{x}
$$
$$
\frac{\partial L }{\partial x} = -k(x-x_{0})-mg
$$
$$
m\ddot{x} + k(x-x_{0}) + mg = 0
$$
$$
m\ddot{x} = -k(x-x_{0})-mg
$$
Be careful how you define positive and negative

Newtonian and Lagrangian mechanics are $\equiv$
 Consider newtons second law
 
 $$
\frac{md^{2}\vec{x}}{dt^{2}} = \vec{F}(\vec{x},\vec{\dot{x}},t)
$$
The general kinetic energy is given by 
$$
T = \frac{1}{2}mv^{2}
$$
Now lets take the time derivative of the velocity derivative
$$
\frac{d}{dt}\left( \frac{\partial T}{\partial\ddot{x}} \right) = m\ddot{x}
$$
We now have the time derivative of the velocity derivative equal to force
$$
\frac{d}{dt} \frac{\partial T }{\partial \ddot{x}} = F
$$
Assuming conservative force 
$$
\vec{F} = -\vec{\nabla}u
$$
So each component is equal to 
$$
F_{x i } = \frac{\partial u }{\partial x_{i}}
$$
And now we rewrite newtons second law: 
$$
\frac{d}{dt} \frac{\partial T }{\partial \dot{x}} + \frac{\partial u }{\partial x} = 0 
$$
Generalized: 
$$
\frac{d}{dt} \frac{\partial T }{\partial \dot{x}_{i}} + \frac{\partial u }{\partial x_{i}} = 0
$$
This leads us to the Euler-Lagrange equation. Cool
	We can say they are equivalent for the cases when the kinetic energy is independent of position. $\frac{dt}{dx_{i}}=0$ and when the potential energy is independent of velocity($\frac{du}{d\dot{x}_{i}}=0$) 
	So $L=T-U$ gives us the same answer
More explicitly: 
$$
\frac{d}{dt} \frac{\partial L }{{\partial} \dot{q_{i}}}-\frac{\partial L }{\partial  q_{i}}
$$
Example Pendulum

Pendulum with length $l$ , mass $m$ and displacement angle $\theta$
Use polar coordinates! Only one Equation of motion  vs 2 

$$
T = \frac{1}{2} m(\dot{x}^{2} + \dot{y}^{2})
$$
$$
u = mgy
$$
$$
L = \frac{1}{2}m(\dot{x}^{2}+\dot{y}^{2}) -mgy
$$
$$
x=l\sin \theta; \ \ \dot{x} = l\dot{\theta}\cos \theta
$$
$$
y=-l\cos \theta ; \ \ \dot{y} = l\dot{\theta}\sin \theta
$$
$$
L = \frac{1}{2}m (l^{2}\dot{\theta}^{2}\cos ^{2}\theta+l^{2}\dot{\theta}^{2}\sin ^{2}\theta) + mgl\cos(\theta)
$$
$$
\sin ^{2}\theta + \cos ^{2}\theta = 1
$$
$$
L = \frac{1}{2}ml^{2}\dot{\theta}^{2} + mgl\cos \theta
$$
$$
\frac{dl}{d\dot{\theta}} = ml^{2}\theta , \ \ \frac{d}{dt}  \frac{dL}{d\dot{\theta}} = ml^{2} \ddot{\theta}
$$
$$
\frac{dl}{d\theta} = -mgl\sin \theta
$$
$$
\frac{d}{dt}  \frac{dl}{d\dot{\theta}} - \frac{dl}{d\theta} = 0
$$
$$
\implies ml^{2}\ddot{\theta}+mgl\sin \theta = 0
$$
$$
\ddot{\theta} = -\frac{g}{l} \sin \theta
$$
Solving using small angle approximation 


## Calculus of Variations 
Based on Hamilton's principle of least action
Consider a dynamical system that moves from point 1 to point 2 within a specified time interval, $dt$. System goes from 1 $\to$ 2 in time $dt$

In all of the paths along which that dynamical system will move along, the actual path which is followed is the one that **minimizes** the **action**. 

What the hell does that mean?
	"The action"
	The combination of kinetic and potential energies, aka the Lagrangian

Hacky sack! 
Point 1 is Prof. martin's hand. Point 2 is Nate's hand. There are an infinite number of paths between these two points, but the minimum action path is taken by the object. 

This is the time integral of the Lagrangian
$$
d \int\limits_{t_{1}}^{t_{2}} (T-U) \, dt = 0 
$$
This is also used in quantum physics. 
$$
J = \int\limits_{t_{1}}^{t_{2}} L(x,\dot{x},t)  \, dt 
$$
$$
dj = 0
$$
The mathematical foundation of Lagrange's equation is the extremum principle

### This is calculus of variations

Given a function $f(x)$, to find an extremum of $f(x)$ we look to see where the first derivative vanishes

$$
\frac{df}{dx}= 0 
$$
Now, we instead want to find the extremum of the integral 
$$
	J = \int\limits_{x_{1}}^{x_{2}} F(y(x),y'(x), x) \, dx 
$$
$$
y'(x) = \frac{dy}{dx}
$$
Rewrite y: $y(\alpha, x)$ 
$$
y(\alpha, x) = y(0,x) +\alpha \eta(x)
$$
When $\alpha = 0$
$$
y(\alpha=0,x) = y(0,x)
$$
This is the function that minimizes J
Constraints 
$\eta(x)$ has a continuous first derivative that vanishes at bounds $x_{1},x_{2}$. 

$$
\frac{d \eta}{dx} \text{ exists}
$$
$$
\eta(x_{1}) = \eta(x_{2}) = 0
$$
So 
$$
y(\alpha, x_{1}) = y(0,x_{1})
$$
$$
y(\alpha, x_{2}) = y(0,x_{2})
$$
With these requirements
$$
J(\alpha) = \int\limits_{x_{1}}^{x_{2}} F(y(\alpha,x),y'(\alpha,x),x) \, dx 
$$
$$
\frac{\partial J}{\partial \alpha}|_{\alpha=0} = 0
$$
Take derivatives 
$$
\frac{dJ}{d\alpha} = \frac{d}{d\alpha} \int\limits_{x_{1}}^{x_{2}} F(y,y',x) \, dx 
$$
$$
=\int\limits_{x_{2}}^{x_{2}} \left[ \frac{\partial F}{\partial y}\frac{\partial y }{\partial \alpha} + \frac{\partial F}{\partial y'} \frac{\partial y'}{\partial \alpha}\right] \, dx 
$$
$$
y = y(0,x) + \alpha \eta(x)
$$
$$
y'(\alpha,x) = \frac{dy}{dx} = \frac{dy(0,x)}{dx} + \alpha \frac{d \eta(x)}{dx}
$$
$$
\frac{dJ}{d\alpha}= \int\limits_{x_{1}}^{x_{2}} \left[ \frac{dF}{dy}\eta(x) + \frac{dF}{dy'} \frac{d \eta(x)}{dx} \right] \, dx 
$$
Now lets use integration by parts for the second term
$$
\int\limits_{x_{1}}^{x_{2}} \frac{dF}{dy'} \frac{d \eta(x)}{dx} \, dx 
$$
$$
u = \frac{dF}{dy'}
$$
$$
du = \frac{d}{dx} \frac{dF}{dy'}
$$
$$
dv = \frac{d \eta}{dx}
$$

$$
v=\eta
$$
$$
\int u \, dv = uv- \int v \, du  
$$
$$
\int\limits_{x_{1}}^{x_{2}} \frac{df}{dy'} \frac{d \eta}{dx} \, dx = \frac{dF}{dy'}\eta |^{x_{2}}_{x_{1}} - \int\limits_{x_{1}}^{x_{2}} \frac{d}{dx} \frac{dF}{dy'} \eta(x) \, dx 
$$
$\eta(x)=0 \ \therefore$ middle term is 0

$$
\frac{dJ}{d\alpha} =\int\limits_{x_{1}}^{x_{2}} \left[ \frac{dF}{dy} \eta(x) - \frac{d}{dx} \frac{dF}{dy'} \eta(x) \right] \, dx 
$$
$$
	=\int\limits_{x_{1}}^{x_{2}} \left[ \frac{dF}{dy} - \frac{d}{dx} \frac{dF}{dy'} \right] \eta(x) \, dx = 0 
$$
Euler Lagrange equation comes from calculus of variations
For non-trivial equations (aka $\eta_{9}x \neq 0$) we find 
$$
\frac{dF}{dy} - \frac{d}{dx} \frac{dF}{dy} =0
$$
Euler Lagrange equation!



